Add exercise.

inductive_type.v
@@ -1,3 +1,5 @@
+Require Import Arith.
+Load CpdtTactics.
 Inductive truth:Set:=Yes|No|Maybe.
 Definition not(b:truth):truth:=
   match b with
@@ -32,10 +34,102 @@ Fixpoint flattern(S:Set)(sl:slist S):list S:=
   match sl with
   | Nil => nil
   | Single s => cons s nil
-  | Concat l r => flattern S l ++ flattern S r
+  | Concat l r => flattern l ++ flattern r
   end.
-Lemma flattern_distributive:forall a b c, flattern a b ++ flattern a c = flattern a (Concat a b c).
+Lemma flattern_distributive:forall (a:Set)(b:slist a)c,
+  flattern b ++ flattern c = flattern (Concat b c).
   reflexivity.
+Qed.
+Inductive binop : Set := Plus | Times.
+Inductive exp : Set :=
+| Var : nat -> exp
+| Const : nat -> exp
+| Binop : binop -> exp -> exp -> exp.
+Definition binopDenote(b:binop):nat->nat->nat:=
+  match b with
+  | Plus => plus
+  | Times => mult
+  end.
+Fixpoint expDenote(f:nat->nat)(e:exp):nat:=
+  match e with
+  | Const n => n
+  | Binop b e1 e2 =>
+      (binopDenote b)
+      (expDenote f e1)
+      (expDenote f e2)
+  | Var n => f n
+  end.
+Inductive folded_exp : Set :=
+| FVar : nat -> folded_exp
+| FConst : nat -> folded_exp
+| FBinop : binop -> noconst -> folded_exp -> folded_exp
+with noconst:Set:=
+| NCVar : nat -> noconst
+| NCBinop: binop -> noconst -> folded_exp -> noconst.
+Fixpoint fold(e:exp):folded_exp:=
+  match e with
+  | Const n => FConst n 
+  | Var n => FVar n
+  | Binop b e1 e2 =>
+      match fold e1 with
+      | FVar n => FBinop b (NCVar n) (fold e2)
+      | FConst l => 
+          match fold e2 with
+          | FVar n => FBinop b (NCVar n)(FConst l)
+          | FConst r => FConst ((binopDenote b)l r)
+          | FBinop bi nc fo => FBinop b (NCBinop bi nc fo) (FConst l)
+          end
+      | FBinop bi nc fo => FBinop b (NCBinop bi nc fo) (fold e2)
+      end
+  end.
+Fixpoint folded_exp_denote(f:nat->nat)(e:folded_exp):nat:=
+  match e with
+  | FConst n => n
+  | FBinop b e1 e2 =>
+      expDenote
+        f
+        (Binop 
+          b
+          (Const (noconst_denote f e1))
+          (Const(folded_exp_denote f e2)))
+  | FVar n => f n
+  end
+with noconst_denote(f:nat->nat)(e:noconst):nat:=
+  match e with
+  | NCVar n => f n
+  | NCBinop b nc fo => 
+      (binopDenote b)(noconst_denote f nc)(folded_exp_denote f fo)
+  end.
+Scheme folded_exp_mut:=Induction for folded_exp Sort Prop
+with noconst_list_mut:=Induction for noconst Sort Prop.
+Lemma binop_comm:forall b l r,binopDenote b l r = binopDenote b r l.
+  destruct b;crush.
+Qed.
+Lemma binop_injec:forall b l n m,n=m->binopDenote b l n = binopDenote b l m.
+  destruct b;crush.
+Qed.
+Lemma optimize_correctness:forall (e:exp)(f:nat->nat),
+  expDenote f e=folded_exp_denote f (fold e).
+  intros.
+  induction e.
+  crush.
+  crush.
+  simpl expDenote.
+  rewrite IHe1.
+  rewrite IHe2.
+  crush.
+  remember (fold e1).
+  remember (fold e2).
+  induction f0.
+  crush.
+  induction f1.
+  crush.
+  apply binop_comm.
+  crush.
+  crush.
+  apply binop_comm.
+  apply binop_injec.
+  crush.
 Qed.
 Inductive I : Type := s : I.
 Inductive O : Type := .
@@ -48,7 +142,7 @@ Definition f(sum:Sum I O):I:=
   end.
 Definition g(i:I):Sum I O:=
   match i with
-    | s => ((inl I)O)i
+    | s => (inl O)i
   end.
 Theorem iso:forall i : I, f(g(i))=i.
   intro.
@@ -61,7 +155,7 @@ Definition pf T(pro:Prod O T):O:=
   end.
 Definition pg T(o:O):Prod O T:=
   match o with end.
-Lemma prod_O_1 : forall(A:Type)(pro:Prod O A),pg A(pf A pro) = pro.
+Lemma prod_O_1 : forall(A:Type)(pro:Prod O A),pg A(pf pro) = pro.
   intros.
   destruct pro.
   destruct o.
